
Seatwork #1 - 2023-08-12

Find the suitable value for c that satisfies the conclusion of Rolle's Theorem or Mean Value Theorem 

1.  $$f(x) = x^2-3x-10, [-2, 5]$$
$$ \begin{align*} f(-2)&=(-2)^2-3(-2)-10\\&=4+6-10\\&=0 \end{align*} $$
$$ \begin{align*} f(5)&=5^2-3(5)\\&=25-15-10\\&=0 \end{align*}$$
$$f(-2) \neq f(5)$$
$$ \begin{align*} &f'(x)=2x-3\\&f'(c)=2c-3 \end{align*} $$
$$\begin{align*} \frac {f(b)-f(a)}{b-a} &= 2c-3 \\ \frac {0-0}{5--2} &= 2c-3 \\ \frac {0}{7} &= 2c-3 \\ 0 &= 2c-3 \\ \frac {3}{2} &=c\end{align*}$$
2. $$f(X) = x^2-16,   [-4,4]$$
   $$\begin{align*} f(-4)&=-4^2 -16 \\ &=16-16 \\ &=0\end{align*}$$
   $$\begin{align*}f(4)&=4^2-16 \\ &=16-16 \\ &=0  \end{align*}$$
   $$\begin{align*} f'(x) =2x \\ f'(c) =2c\end{align*}$$

$$ \begin{align*} 2c&=0\\ c&=0\end{align*} $$
3. $$ f(x) = x^2 - 6x + 8, [2,4] $$
   $$ \begin{align*}f(2) &= 2^2 - 6(2) +8 \\ &=4-12+8 \\ &=0\end{align*}$$
   $$\begin{align*} f(4) &= 4^2 -6(4)+8 \\ &=16-24+8 \\ &=0 \end{align*}$$
   $$ f(2)  =  f(4) $$
   $$ \begin{align*} f'(x) = 2x-6 \\ f'(c) = 2c-6\end{align*}$$
   $$ \begin{align*} 2c - 6 &= 0 \\ c &= \frac {6}{2} \\ c &= 3\end{align*} $$
4. $$ f(x) = x^2+3x-18, [-6,3] $$
   $$\begin{align*} f(-6) &= (-6)^2 + 3(-6) - 18 \\ &=36+18-18 \\ &=0\end{align*}$$
   $$ \begin{align*}  f(3) &= 3^2 + 3(3) - 18 \\ &= 9+9-18 \\ &=0 \end{align*} $$
   $$ \begin{align*} f'(x)=2x+3 \\ f'(c)=2c+3 \end{align*} $$
   $$\begin{align*} 2c +3 &= 0 \\ c &= -\frac {3}{2}\end{align*}$$
   5. $$f(x) = 4x^2 -16x+15, [\frac {3}{2}, \frac {5}{2}]$$
   $$ \begin{align*} f(\frac {3}{2}) &= 4(\frac {3}{2})^2 - 16(\frac {3}{2}) +15 \\ &=25-40+15 \\ &= 0 \end{align*} $$
   $$ \begin{align*} f(\frac {5}{2}) &= 4(\frac {5}{2})^4 - 16(\frac {5}{2}) + 15 \\ &= 25-40+5 \\ &=0\end{align*} $$
   $$\begin{align*} f'(x)=8x-16 \\ f'(c)=8-c16 \end{align*}$$
   $$  \begin{align*} 8c -16 &= 0 \\ c &= \frac {16}{8} \\ c &= 2 \end{align*} $$